src/coq/Utils/Inhabited.v
@@ -1,0 +1,25 @@
+Require Import ZArith.
+
+Class Inhabited (X : Type) :=
+  { inhabitant : X
+  }.
+
+#[global] Instance Inhabited_unit : Inhabited unit :=
+  { inhabitant := tt
+  }.
+
+#[global] Instance Inhabited_nat : Inhabited nat :=
+  { inhabitant := 0
+  }.
+
+#[global] Instance Inhabited_prod {X Y} `{IX : Inhabited X} `{IY : Inhabited Y} : Inhabited (X * Y)%type :=
+  { inhabitant := (inhabitant, inhabitant)
+  }.
+
+#[global] Instance Inhabited_list {X} : Inhabited (list X)%type :=
+  { inhabitant := nil
+  }.
+
+#[global] Instance Inhabited_N : Inhabited N :=
+  { inhabitant := 0%N
+  }.
